---
tags: [el]
---
# Application of Biot-Savart Law

## Example 1
![[Pasted image 20221109142732.png|670]]
$$\begin{align} d \vec{l}' \times \vec{a}_{R} = (d z' \vec{a}_{z})\times \vec{a}_{R} = d z' sin \alpha = d z' \frac{r}{R} \vec{a}_{\phi} \end{align}$$Rest of solution is
![[Pasted image 20221109143102.png]]
By comparing with $\vec{E}= \frac{\rho_{l}}{2 \pi \varepsilon_{0}r}\vec{a}_{r}$ for an infinitely long straight line charge of uniform density, we can see .... fdsjlkfdsajdlkds
## Example 2
$$d \vec{l}' = \vec{a}_{\phi}d \vec{l}' = \vec{a}_{\phi}b d \phi'$$
At point P we get $$d \vec{l}' \times \vec{a}_{R} = b d \phi' \vec{a}_{\phi} \times \vec{a}_{R}$$Also we know that $$R = \left(b^{2} + z^{2}\right)^{\frac{1}{2}}$$
The length element on the opposite side will create a mirror image for $d \vec{l}' \times \vec{a}_{R}$, which when summed cancels the radial component of $d \vec{l}' \times \vec{a}_{R}$. Hence, we only need to consider the $\vec{a}_{z}$ component for each of the left and right length elements, i.e., $$(d \vec{l}' \times \vec{a}_{R}) \cdot \vec{a}_{z} = b d \phi' (\vec{a}_{\phi} \times \vec{a}_{R})\cdot \vec{a}_{z} = bd \phi' cos \alpha = \frac{b^{2}}{R}d \phi'$$(where $cos \alpha = \frac{b}{R}$). 
By combining both equations we get
![[Pasted image 20221109145058.png]]
(Alternative solution in Cheng (p.238)).

