$$
\begin{align} \begin{cases} z_{0} = e^{j \frac{\pi}{2}} \\ z^*_{{0}}= e^{-j \frac{\pi}{2}} \end{cases} \end{align}
$$
and we can now write 
$$
\begin{align} H_{1}(z) = \left( 1-e^{j \frac{\pi}{2}}z^{-1} \right)\left(1-e^{-j \frac{\pi}{2}}z^{-1}\right)= ... = \frac{1+z^{2}-2cos(\frac{\pi}{2})z}{z^{2}} \end{align}
$$


$$\begin{align} H_{2}(z) = \frac{(z-e^{j \frac{\pi}{2}})(z-e^{-j \frac{\pi}{2}})}{(z-0,95e^{j \frac{\pi}{2}})(z-0,95e^{-j \frac{\pi}{2}})}  = \frac{1-(2cos \frac{\pi}{2})z^{-1}+z^{-2}}{1-(2 \cdot 0,95 \cdot cos \frac{\pi}{2})z^{-1}+0,95^{2} \cdot z^{-2}}\end{align}$$